Progress on proof of epoch persistency

src/examples/epoch_persistency.v
@@ -13,26 +13,26 @@ From self.base Require Import primitive_laws class_instances crash_borrow.
 From self.high Require Import proofmode wpc_proofmode.
 From self.high Require Import dprop resources crash_weakestpre weakestpre
      weakestpre_na weakestpre_at recovery_weakestpre lifted_modalities modalities crash_borrow
-     post_crash_modality protocol no_buffer abstract_state_instances locations protocol.
+     post_crash_modality protocol no_buffer abstract_state_instances locations protocol if_rec.
 From self.high.modalities Require Import fence.
 
 Section program.
 
-  Definition leftProg (x : loc) : expr :=
+  Definition left_prog (x : loc) : expr :=
     #x <-_AT #2.
 
-  Definition rightProg (x y z : loc) : expr :=
+  Definition right_prog (x y z : loc) : expr :=
     #x <-_AT #1 ;;
     let: "a" := !_AT #x in
     Flush #x ;;
-    if: "a" = #2
+    (if: "a" = #2
     then #y <-_NA #1
-    else #() ;;
+    else #()) ;;
     Fence ;;
     #z <-_NA #1.
 
   Definition prog (x y z : loc) : expr :=
-    Fork (leftProg x) ;; rightProg x y z.
+    Fork (left_prog x) ;; right_prog x y z.
 
   Definition recovery x y z : expr :=
     if: (!_NA #y = #true) && (!_NA #z = #true)
@@ -41,7 +41,34 @@ Section program.
 
 End program.
 
-Definition x_state := option (bool + bool).
+(* Definition x_state := option (bool + bool). *)
+Inductive x_state := x_zero | x_one | x_two.
+
+Instance x_state_eqdecision : EqDecision x_state.
+Proof. Admitted.
+
+Instance x_state_countable : Countable x_state.
+Proof. Admitted.
+
+Definition x_state_order (x1 x2 : x_state) : Prop :=
+  match x1, x2 with
+    x_zero, _ => True
+  | _, x_zero => False
+  | _, _ => True
+  end.
+
+Program Instance x_state_abstract_state :
+  AbstractState x_state := { abs_state_relation := x_state_order }.
+Next Obligation.
+  split; repeat intros [| |]; done.
+Qed.
+
+Definition x_state_to_nat (x : x_state) : nat :=
+  match x with
+    x_zero => 0
+  | x_one => 1
+  | x_two => 2
+  end.
 
 (* One shot resource algebra that we use in this example. *)
 Definition one_shotR := csumR (exclR unitO) (agreeR (leibnizO x_state)).
@@ -58,48 +85,27 @@ Section proof.
 
   Context (x y z : loc) (γag : gname) (γtok : gname).
 
-  (* Protocol for [x]. *)
-
-  Definition zero : x_state := None.
-  Definition one_l : x_state := Some (inl false).
-  Definition one_r : x_state := Some (inr false).
-  Definition two_l : x_state := Some (inl true).
-  Definition two_r : x_state := Some (inr true).
-
-  Definition x_state_to_nat (s : x_state) : nat :=
-    match s with
-      None => 0
-    | Some (inl false) => 1
-    | Some (inr false) => 1
-    | Some (inl true) => 2
-    | Some (inr true) => 2
-    end%I.
-
   Definition tok0 : dProp Σ := ⎡ own γtok (GSet {[ 0 ]}) ⎤.
   Definition tok1 : dProp Σ := ⎡ own γtok (GSet {[ 1 ]}) ⎤.
   Definition tok2 : dProp Σ := ⎡ own γtok (GSet {[ 2 ]}) ⎤.
-  Definition tokFin1 : dProp Σ := ⎡ own γtok (GSet {[ 3 ]}) ⎤.
-  Definition tokFin2 : dProp Σ := ⎡ own γtok (GSet {[ 4 ]}) ⎤.
+
+  (* Protocol for [x]. *)
 
   Program Definition prot_x := {|
     pred s v _ := (
       ⌜ v = #(x_state_to_nat s) ⌝ ∗
-      (* (⌜ s = zero ⌝ ∨ *)
-      (*   ⌜ s = two_l ⌝ ∗ tok2 ∗ (tokFin1 ∨ tokFin2) ∨ *)
-      (*   ⌜ s = one_l ⌝ ∗ tok1 ∗ tokFin1 ∨ *)
-      (*   ⌜ s = one_r ⌝ ∗ tok1 ∗ (tokFin1 ∨ tokFin2) ∨ *)
-      (*   ⌜ s = two_r ⌝ ∗ tok2 ∗ tokFin2))%I *)
       match s with
-        None => tok0
-      | Some (inl true) => tok2 ∗ (tokFin1 ∨ tokFin2)
-      | Some (inl false) => tok1 ∗ tokFin1
-      | Some (inr false) => tok1 ∗ (tokFin1 ∨ tokFin2)
-      | Some (inr true) => tok2 ∗ tokFin2
+        x_zero => tok0
+      | x_one => tok1
+      | x_two => tok2
       end)%I
     ;
     bumper b := b;
   |}.
-  Next Obligation. iIntros (? [[[|]|[|]]|] ?) "H"; simpl; iCrashFlush; done. Qed.
+  Next Obligation.
+    iIntros (? [| |] ?) "H"; simpl; iCrashFlush; done.
+  Qed.
+  Next Obligation. Admitted.
 
   (* Protocol for [y]. *)
 
@@ -107,7 +113,10 @@ Section proof.
     {| pred (b : bool) (v : val) _ :=
         match b with
           false => ⌜ v = #0 ⌝
-        | true => ⌜ v = #1 ⌝ ∗ ⎡ own γag (Shot two_r) ⎤
+        | true =>
+            ⌜ v = #1 ⌝ ∗
+            ⎡ own γag (Shot x_two) ⎤
+            (* (flush_lb x prot_x x_two -∗ x ↦_AT^{prot_x} [x_zero; x_one; x_two]) *)
         end%I;
       bumper b := b; |}.
   Next Obligation. Admitted.
@@ -119,89 +128,277 @@ Section proof.
     {| pred (b : bool) (v : val) _ :=
         match b with
           false => ⌜ v = #0 ⌝
-        | true => ⌜ v = #1 ⌝ ∗ ∃ n, ⎡ own γag (Shot n) ⎤ ∗ flush_lb x prot_x n
+        | true =>
+            ⌜ v = #1 ⌝ ∗
+            ∃ n, ⎡ own γag (Shot n) ⎤ ∗
+                 flush_lb x prot_x n ∗
+                 ((⌜ n = x_one ⌝ ∗ x ↦_AT^{prot_x} [x_zero; x_one]) ∨
+                  (⌜ n = x_two ⌝ ∗ x ↦_AT^{prot_x} [x_zero; x_one; x_two]))
         end%I;
       bumper b := b; |}.
-  Next Obligation. Admitted.
-  Next Obligation. Admitted.
+  Next Obligation.
+    iIntros (? [|] v); last first.
+    { iIntros "H". iCrashFlush. done. }
+    iIntros "(-> & (%s & shot & fLb & [[A B]|[A B]]))".
+    - admit.
+    - admit.
+  Admitted.
   Next Obligation. Admitted.
 
   Definition crash_condition {hD : nvmDeltaG} : dProp Σ :=
-    ∃ (yb bz : bool),
-      ⎡ is_at_loc x ⎤ ∗
-      persist_lb x prot_x None ∗
+    ∃ xss yss zss,
+      (* x *)
+      persist_lb x prot_x x_zero ∗
+      x ↦_AT^{prot_x} xss ∗
       (* y *)
       persist_lb y prot_y false ∗
-      y ↦_{prot_y} [yb] ∗
+      y ↦_{prot_y} yss ∗
       (* z *)
       persist_lb z prot_z false ∗
-      z ↦_{prot_z} [bz].
+      z ↦_{prot_z} zss.
 
-  Definition left_crash_condition {hD : nvmDeltaG} : dProp Σ :=
-    ⎡ is_at_loc x ⎤ ∗ persist_lb x prot_x None.
+  (* Definition left_crash_condition {hD : nvmDeltaG} : dProp Σ := *)
+  (*   ∃ xss xs, *)
+  (*     x ↦_AT^{prot_x} (xss ++ [xs]) ∗ *)
+  (*     persist_lb x prot_x xs. *)
 
- (*  Lemma left_prog_spec : *)
- (*    tok2 -∗ tokFin1 -∗ ⎡ is_at_loc x ⎤ -∗ persist_lb x prot_x None -∗ *)
- (*    WPC leftProg x @ ⊤ *)
- (*      {{ v, store_lb x prot_x two_l ∨ store_lb x prot_x two_r }} *)
- (*      {{ <PC> _, True }}. *)
- (*  Proof. *)
- (*    iIntros "tok tokFin #atLoc #perLb". *)
- (*    rewrite /leftProg. *)
- (*    iApply wpc_atomic_no_mask. *)
- (*    iSplit. { iCrash. done. } *)
- (*    iApply ( *)
- (*        wp_store_at_strong _ (λ s, ⌜ s = two_l ∨ s = two_r ⌝)%I with "[$atLoc tok tokFin]"). *)
- (*    { iDestruct (persist_lb_to_store_lb with "perLb") as "$". *)
- (*      iIntros (s_l v_l le). *)
- (*      (* [s_l] can either be [zero] or [one_r]. *) *)
- (*      destruct (decide (s_l = zero)) as [->|neq]. *)
- (*      - iExists two_l. *)
- (*        iSplit. { *)
- (*          iIntros (? [[[|]|[|]]|] ??) "H1 [-> H2]"; simpl. *)
- (*          * admit. *)
- (*          * admit. *)
- (*          * admit. *)
- (*          * admit. *)
- (*          * admit. } *)
- (* (* simplify_eq. *) *)
- (*          (* iSplit; first done. *) *)
- (*          (* admit. } *) *)
- (*        iSplitL "". { iModIntro. iIntros "$". rewrite left_id. iAccu. } *)
- (*        iIntros "_". *)
- (*        iSplit; last (iLeft; done). *)
- (*        iSplitPure; first done. *)
- (*        iRight. iLeft. iFrame. done. *)
- (*      - iExists two_r. *)
- (*        iSplitL "". { admit. } *)
- (*        simpl. iSplitPure; first done. *)
- (*        iRight. iRight. iRight. iRight. iFrame. done. *)
- (*      } *)
- (*  Qed. *)
+  Lemma left_prog_spec :
+    tok2 -∗
+    persist_lb x prot_x x_zero -∗
+    x ↦_AT^{prot_x} [x_zero] -∗
+    WPC left_prog x @ ⊤
+      {{ v, x ↦_AT^{prot_x} [x_zero; x_two] }}
+      {{ <PC> _, True }}.
+  Proof.
+    iIntros "tok #perLb xPts".
+    rewrite /left_prog.
+    iApply wpc_atomic_no_mask.
+    iSplit. { iCrash. done. }
+    iApply (wp_store_at _ [] _ x_two with "[$xPts $tok]").
+    { iSplitPure; first done.
+      iSplitPure; first done.
+      (* iDestruct (persist_lb_to_store_lb _ _ x_two with "perLb") as "$". *)
+      iIntros (v_i s_l v_l le).
+      (* [s_l] can either be [x_zero] or [one_r]. *)
+      destruct s_l; simpl.
+      - iIntros "((-> & tok1) & (? & tok2) & (-> & tok3))".
+        iDestruct (own_valid_2 with "tok1 tok3") as %hi%gset_disj_valid_op.
+        set_solver.
+      - iIntros "?". done.
+      - iIntros "((-> & tok1) & (? & tok2) & (-> & tok3))".
+        done. }
+    iIntros "!> pts".
+    iSplit. { iModIntro. iCrash. done. }
+    iModIntro. iApply "pts".
+  Qed.
+
+  Lemma prove_crash_condition xss yss zss :
+    (* x *)
+    persist_lb x prot_x x_zero -∗
+    x ↦_AT^{prot_x} xss -∗
+    (* y *)
+    persist_lb y prot_y false -∗
+    y ↦_{prot_y} yss -∗
+    (* z *)
+    persist_lb z prot_z false -∗
+    z ↦_{prot_z} zss -∗
+    <PC> _, crash_condition.
+  Proof.
+    iIntros "xPLb xPts yPLb yPts zPLb zPts".
+    iCrash.
+    iDestruct "xPLb" as "[xPLb (%xsC & % & #xCrash)]".
+    iDestruct "yPLb" as "[yPLb (%ysC & % & #yCrash)]".
+    iDestruct "zPLb" as "[zPLb (%zsC & % & #zCrash)]".
+    iDestruct (crashed_in_if_rec with "xCrash xPts") as (xsC') "[xCrash' disj]".
+    iDestruct (crashed_in_agree with "xCrash xCrash'") as %<-.
+    iDestruct "disj" as "[L|R]"; last first.
+  Admitted.
+    (* { iDestruct "R" as (? ([= eq] & le & neq)) "_". *)
+    (*   exfalso. *)
+    (*   destruct xsC; done. } *)
+    (* iDestruct "L" as (xss xs pre le) "xPts". *)
+    (* rewrite /crash_condition. *)
+    (* iExists ((λ b : x_state, b) <$> xss), xs. iExistsN. *)
+    (* iSplitL "xPts". { *)
+    (* iFrame "xPts". *)
+  (* Qed. *)
+
+  Ltac solve_cc :=
+    iApply (prove_crash_condition with "xPLb xPts yPLb yPts zPLb zPts").
 
   Lemma right_prog_spec :
-    tokFin1 -∗ tok2 -∗
+    tok1 -∗
     ⎡ pre_borrow ⎤ -∗
+    ⎡ own γag Pending ⎤ -∗
     (* x *)
-    ⎡ is_at_loc x ⎤ -∗
-    persist_lb x prot_x None -∗
+    persist_lb x prot_x x_zero -∗
+    x ↦_AT^{prot_x} [x_zero] -∗
     (* y *)
     persist_lb y prot_y false -∗
     y ↦_{prot_y} [false] -∗
     (* z *)
     persist_lb z prot_z false -∗
     z ↦_{prot_z} [false] -∗
-    WPC prog x y z @ ⊤
+    WPC right_prog x y z @ ⊤
       {{ v, True }}
       {{ <PC> _, crash_condition }}.
-  Proof. Admitted.
+  Proof.
+    iIntros "tok1 pre shot xPLb xPts yPLb yPts zPLb zPts".
+    rewrite /right_prog.
+    wpc_bind (_ <-_AT _)%E.
+    wpc_atomic; first solve_cc.
+    iApply (wp_store_at _ [] _ x_one with "[$xPts tok1]").
+    { iSplitL "tok1". { simpl. iFrame "tok1". done. }
+      iSplitPure; first done.
+      iIntros (? sC ??).
+      destruct sC; simpl.
+      - iIntros "((-> & tok1) & (? & tok2) & (-> & tok3))".
+        iDestruct (own_valid_2 with "tok1 tok3") as %hi%gset_disj_valid_op.
+        set_solver.
+      - iIntros "?". done.
+      - iIntros "((-> & tok1) & (? & tok2) & (-> & tok3))".
+        done. }
+    iNext.
+    iIntros "xPts".
+    iSplit; iModIntro; first solve_cc.
+    wpc_pures; first solve_cc.
+    wpc_bind (!_AT _)%E.
+    wpc_atomic; first solve_cc.
+    iApply (wp_load_at _ _ _
+             (λ v, ⌜ v = #1 ⌝)%I
+             (λ s v, ⌜ s = x_two ∧ v = #2 ⌝)%I with "[xPts]").
+    { iFrame "xPts".
+      iSplit.
+      - iIntros (??).
+        (* iExists (λ s, ⌜ s = x_two ⌝)%I. *)
+        admit.
+      - iIntros (vs vL sL).
+        iExists ⌜ sL = x_two ⌝%I.
+        iIntros (sLe).
+        iSplitL.
+        { iIntros "L".
+          iDestruct (big_sepL2_cons_inv_l with "L") as (???) "[[-> tok0] L]".
+          iDestruct (big_sepL2_cons_inv_l with "L") as (bin go cat) "[[-> tok1] L]".
+          iDestruct (big_sepL2_cons_inv_l with "L") as (ho hi hip) "[[eq tok2] L]".
+          iDestruct (big_sepL2_nil_inv_l with "L") as %->.
+          simpl.
+          simplify_eq.
+          assert (vL = ho) as <-. { admit. }
+          destruct sL; first done; last done.
+          iDestruct (own_valid_2 with "tok1 tok2") as %hi%gset_disj_valid_op.
+          set_solver. }
+        iIntros (->).
+        iModIntro.
+        simpl.
+        iIntros "(-> & $)".
+        done. }
+    iIntros "!>" (?) "H".
+    rewrite post_fence_flush_free.
+    iAssert (∃ xss xs,
+              x ↦_AT^{ prot_x} (xss ++ [xs]) ∗
+              ((⌜ vL = #1 ∧ xss = [x_zero] ∧ xs = x_one ⌝) ∨
+              (⌜ vL = #2 ∧ xss = [x_zero; x_one] ∧ xs = x_two ⌝)))%I
+      with "[H]" as (xss xs) "[xPts disj]".
+      { iDestruct "H" as "[(%sL & xPts & eq)|(xPts & ->)]".
+        - iExists _, _.
+          rewrite post_fence_flush_free.
+          iDestruct "eq" as %(-> & ->).
+          iFrame "xPts".
+          iRight.
+          done.
+        - iExists _, _.
+          iFrame "xPts".
+          iLeft.
+          done. }
+    iSplit; first (iModIntro; solve_cc).
+
+    (* Let us now do the irrevesible irrevocable forever-done action that is
+     * firing the one-shot ghost state. *)
+    iMod (own_update with "shot") as "shot".
+    { apply (cmra_update_exclusive (Shot xs)). done. }
+    iDestruct "shot" as "#shot".
+
+    iModIntro.
+    wpc_pures; first solve_cc.
+
+    wpc_bind (Flush _)%E.
+    iApply wpc_atomic_no_mask.
+    iSplit; first solve_cc.
+    iApply (wp_flush_at with "xPts").
+    iIntros "!> (xPts & #fLb & _)".
+    iSplit; iModIntro; first solve_cc.
+    wpc_pures; first solve_cc.
+    (* This is that spot where we hit a fork in the road. To take the if branch
+     * or not to take the if branch. That is the question. *)
+    iDestruct "disj" as "[(-> & -> & ->) | (-> & -> & ->)]".
+    - rewrite bool_decide_false //.
+      wpc_pures; first solve_cc.
+      (* fence *)
+      wpc_bind Fence.
+      iApply wpc_atomic_no_mask.
+      iSplit; first solve_cc.
+      iApply wp_fence. do 2 iModIntro.
+      iSplit; iModIntro; first solve_cc.
+      wpc_pures; first solve_cc.
+      (* write to [z] *)
+      iApply wpc_atomic_no_mask.
+      iSplit; first solve_cc.
+      iDestruct "xPts" as "#xPts".
+      iApply (wp_store_na _ _ _ _ _ true with "[$zPts]"); eauto.
+      { simpl.
+        iSplitPure; first done.
+        iExists x_one.
+        iFrame "shot fLb".
+        iLeft.
+        iSplitPure; first done.
+        iFrame "xPts". }
+      iIntros "!> zPts".
+      iSplit; iModIntro; first solve_cc.
+      done.
+    - rewrite bool_decide_true //.
+      wpc_pures; first solve_cc.
+
+      wpc_bind (_ <-_NA _)%E.
+      (* Write to y *)
+      iApply wpc_atomic_no_mask.
+      iSplit; first solve_cc.
+      iApply (wp_store_na _ _ _ _ _ true with "[$yPts]");
+        first done;
+        first done.
+      { simpl. iFrame "shot". done. }
+      iIntros "!> yPts".
+      iSplit; iModIntro; first solve_cc.
+
+      wpc_pures; first solve_cc.
+
+      wpc_bind Fence.
+      iApply wpc_atomic_no_mask.
+      iSplit; first solve_cc.
+      iApply wp_fence. do 2 iModIntro.
+      iSplit; iModIntro; first solve_cc.
+
+      wpc_pures; first solve_cc.
+      (* write to [z] *)
+      iApply wpc_atomic_no_mask.
+      iSplit; first solve_cc.
+      iDestruct "xPts" as "#xPts".
+      iApply (wp_store_na _ _ _ _ _ true with "[$zPts]"); eauto.
+      { simpl.
+        iSplitPure; first done.
+        iExists x_two.
+        iFrame "shot fLb".
+        iRight.
+        iSplitPure; first done.
+        iFrame "xPts". }
+      iIntros "!> zPts".
+      iSplit; iModIntro; first solve_cc.
+      done.
+  Admitted.
 
   Lemma prog_spec :
     tok1 -∗ tok2 -∗
-    tokFin1 -∗ tokFin2 -∗
     ⎡ pre_borrow ⎤ -∗
     (* x *)
-    ⎡ is_at_loc x ⎤ -∗
     persist_lb x prot_x None -∗
     (* y *)
     persist_lb y prot_y false -∗
